# Khan/khan-exercises

Fetching contributors…
Cannot retrieve contributors at this time
290 lines (262 sloc) 7.09 KB
 Order of operations
randRange(1, 10) randRange(1, 10) randRange(1, 10) randRange(1, 10) randRange(1, 10)

Simplify the following expression.

A + (B \times C)

A+B*C

= A + (B*C)

= A + B*C

= A+B*C

A + B \times C

A+B*C

= A + B*C

= A+B*C

A \times (B + C)

A*(B+C)

= A \times B+C

= A*(B+C)

A + (\dfrac{B*C}{C})

A+B

= A + (B)

= A + B

= A+B

A + \dfrac{B*C}{C}

A+B

= A + B

= A+B

\dfrac{ (A*(B+C)) }{ B + C }

A

= \dfrac{ (A*(B+C)) }{ ((B+C)) }

= \dfrac{ (A*(B+C)) }{ B+C }

= A

\dfrac{ (A*(B-C)) }{ (B - C) }

A

= \dfrac{ (A*(B-C)) }{ ((B-C)) }

= \dfrac{ (A*(B-C)) }{ B-C }

= A

(A + (B - C \times D)) \times E

(A+(B-(C*D)))*E

= (A + (B - (C*D))) \times E

= (A + ((B-(C*D)))) \times E

= (A + (B-(C*D))) \times E

= ((A+(B-(C*D)))) \times E

= (A+(B-(C*D))) \times E

= (A+(B-(C*D)))*E

A + (B - C \times D) \times E

A+((B-(C*D))*E)

= A + (B - (C*D)) \times E

= A + ((B-(C*D))) \times E

= A + ((B-(C*D))*E)

= A+((B-(C*D))*E)

A - B \times C + \dfrac{ (D*E) }{ E }

A-B*C+D

= A - B \times C + D

= A - (B*C) + D

= (A-B*C) + D

= A-B*C+D

A \times B + C \times \dfrac{ (D*E) }{ E }

(A*B)+(C*D)

= A \times B + C \times D

= (A*B) + C \times D

= (A*B) + (C*D)

= (A*B)+(C*D)

(A + B \times C) - D \times E

(A+B*C)-(D*E)

= (A + (B*C)) - D \times E

= (A+(B*C)) - D \times E

= (A+(B*C)) - (D*E)

= (A+B*C)-(D*E)

Something went wrong with that request. Please try again.